Lemmas about Is_variable_in.

DataflowSyntax.v
@@ -379,6 +379,15 @@ Inductive Is_memory_in_eq : ident -> equation -> Prop :=
 Definition Is_memory_in (x: ident) (eqs: list equation) : Prop :=
   List.Exists (Is_memory_in_eq x) eqs.
 
+Lemma Is_memory_in_eq_dec:
+  forall x eq, {Is_memory_in_eq x eq}+{~Is_memory_in_eq x eq}.
+Proof.
+  destruct eq as [y cae|y f lae|y v0 lae];
+  (destruct (ident_eq_dec x y) as [xeqy|xneqy];
+     [ rewrite xeqy; left; constructor | right; inversion 1; auto])
+   || (right; inversion_clear 1).
+Qed.
+
 Lemma In_fold_left_memory_eq:
   forall x eqs m,
     PS.In x (List.fold_left memory_eq eqs m)
@@ -447,7 +456,7 @@ Proof.
   apply Is_memory_in_memories.
 Qed.
 
-Fixpoint variable_eq (vars: PS.t) (eq: equation) : PS.t :=
+Fixpoint variable_eq (vars: PS.t) (eq: equation) {struct eq} : PS.t :=
   match eq with
   | EqDef x _   => PS.add x vars
   | EqApp x _ _ => PS.add x vars
@@ -464,6 +473,78 @@ Inductive Is_variable_in_eq : ident -> equation -> Prop :=
 Definition Is_variable_in (x: ident) (eqs: list equation) : Prop :=
   List.Exists (Is_variable_in_eq x) eqs.
 
+Lemma Is_variable_in_eq_dec:
+  forall x eq, {Is_variable_in_eq x eq}+{~Is_variable_in_eq x eq}.
+Proof.
+  intros x eq.
+  destruct eq as [y cae|y f lae|y v0 lae];
+    match goal with
+    | |- context Is_variable_in_eq [EqFby _ _ _] => right; inversion 1
+    | _ => (destruct (ident_eq_dec x y) as [xeqy|xneqy];
+            [ rewrite xeqy; left; constructor
+            | right; inversion 1; auto])
+    end.
+Qed.
+
+Lemma In_fold_left_variable_eq:
+  forall x eqs m,
+    PS.In x (List.fold_left variable_eq eqs m)
+    <-> PS.In x (List.fold_left variable_eq eqs PS.empty) \/ PS.In x m.
+Proof. (* TODO: There must be a way to get auto to do all of this? *)
+  induction eqs as [|eq].
+  - split; auto.
+    destruct 1 as [H|].
+    apply not_In_empty in H; contradiction.
+    auto.
+  - split; [ intro H; simpl; rewrite IHeqs
+           | destruct 1 as [H|H]; apply IHeqs];
+    solve [
+        simpl in H; apply IHeqs in H; destruct H;
+        [ intuition
+        | destruct eq; try (apply PS.add_spec in H; destruct H);
+          match goal with
+          | H:x=_ |- _ => rewrite H; simpl; rewrite PS.add_spec; intuition
+          | _ => apply not_In_empty in H; contradiction
+          | _ => intuition
+          end ]
+      | right; destruct eq; try apply PS.add_spec; intuition
+      ].
+Qed.
+
+Lemma Is_variable_in_variables:
+  forall x eqs,
+    PS.In x (variables eqs)
+    <-> Is_variable_in x eqs.
+Proof.
+  unfold variables, Is_variable_in.
+  induction eqs as [ eq | eq ].
+  - rewrite List.Exists_nil; split; intro H;
+    try apply not_In_empty in H; contradiction.
+  - simpl.
+    rewrite In_fold_left_variable_eq.
+    split.
+    + rewrite List.Exists_cons.
+      destruct 1. intuition.
+      destruct eq; try (apply not_In_empty in H; intuition);
+      (simpl in H; apply PS.add_spec in H; destruct H;
+       [ rewrite H; left; constructor
+       | apply not_In_empty in H; contradiction ]).
+    + intro H; apply List.Exists_cons in H; destruct H.
+      destruct eq; try inversion H;
+      (right; apply PS.add_spec; intuition).
+      left; apply IHeqs; apply H.
+Qed.
+
+Lemma Is_variable_in_dec:
+  forall x eqs, {Is_variable_in x eqs}+{~Is_variable_in x eqs}.
+Proof.
+  intros x eqs.
+  apply Bool.reflect_dec with (b := PS.mem x (variables eqs)).
+  apply Bool.iff_reflect.
+  rewrite PS.mem_spec.
+  symmetry.
+  apply Is_variable_in_variables.
+Qed.
 
 
 Fixpoint defined_eq (defs: PS.t) (eq: equation) {struct eq} : PS.t :=
@@ -483,6 +564,16 @@ Inductive Is_defined_in_eq : ident -> equation -> Prop :=
 
 Definition Is_defined_in (x: ident) (eqs: list equation) : Prop :=
   List.Exists (Is_defined_in_eq x) eqs.
+
+Lemma Is_defined_in_eq_dec:
+  forall x eq, {Is_defined_in_eq x eq}+{~Is_defined_in_eq x eq}.
+Proof.
+  intros x eq.
+  destruct eq as [y cae|y f lae|y v0 lae];
+    (destruct (ident_eq_dec x y) as [xeqy|xneqy];
+     [ rewrite xeqy; left; constructor
+     | right; inversion 1; auto]).
+Qed.
 
 Lemma In_fold_left_defined_eq:
   forall x eqs m,
